More

dataplane/Base_Op_Proofs_Dis.thy
@@ -3,14 +3,12 @@ theory Base_Op_Proofs_Dis
 imports
     "HOL-ex.Sketch_and_Explore" 
     Timely_Infrastructure_Dis
-    "Examples/Set_op"
     "Examples/Tmap_op"
 begin
 
 lemma set_mset_cset[simp]: "rcset (acset (set_mset xs)) = set_mset xs"
   apply(rule acset_inverse)
   using countable_finite by blast
-
 
 (* set'_op *)
 
@@ -67,76 +65,14 @@ lemma step_set_op_intro_Tau_2[intro]:
   apply (metis (no_types, lifting) IO.distinct(5) IO.simps(6) cimageI cinsertI1 op.simps(20) step.simps step_choicesE)
   done
 
-
-(* set'_op that can take input
-corec set'_op :: "('a \<times> 'b) multiset \<Rightarrow> ('c, 'a, 'b) op \<Rightarrow> ('c, 'a, 'b) op" where
-  "set'_op S op = choice2
-  (Choice (cimage (\<lambda> op. case op of
-     Write op p x \<Rightarrow> Silent (set'_op (add_mset (p, x) S) op) 
-   | Silent op \<Rightarrow> Silent (set'_op S op)
-   | Read p f \<Rightarrow> Read p ((set'_op S) o f)
-   ) (choices op))
-   )
-  (Choice (cimage (\<lambda> (p, x). Write (set'_op (remove1_mset (p, x) S) op) p x) ((acset o set_mset) S)))"
-
-lemma step_set'_op_elim:
-  assumes "step io (set'_op S op) op'"
-  obtains p x where "io = Out p x" "(p, x) \<in># S" "op' = set'_op (remove1_mset (p, x) S) op"
-  | op'' where "io = Tau" "step Tau op op''" "op' = set'_op S op''"
-  | p x op'' where "io = Tau" "step (Out p x) op op''" "op' = set'_op (add_mset (p, x) S) op''"
-  | p x op'' where "io = Inp p x" "step (Inp p x) op op''" "op' = set'_op S op''"
-  using assms apply -
-  apply atomize_elim
-  apply (subst (asm) set'_op.code)
-  by (auto del: disjCI split: op.splits simp flip: cin.rep_eq; hypsubst_thin?)
-     (fastforce+)
-
-lemma step_set'_op_intro_Out[intro]:
-  "io = Out p x \<Longrightarrow>
-   (p, x) \<in># S \<Longrightarrow>
-   op' = set'_op (remove1_mset (p, x) S) op \<Longrightarrow>
-   step io (set'_op S op) op'"
-  apply (subst set'_op.code)
-  apply (clarsimp del: disjCI split: op.splits simp add: comp_def simp flip: cin.rep_eq; hypsubst_thin?)
-  apply(rule Write_in_choices_step)
-  by(simp add: Bex_def)
-
-
-lemma step_set'_op_intro_Tau_1[intro]:
-  "step (Out p x) op op'' \<Longrightarrow>
-   io = Tau \<Longrightarrow>
-   op' = set'_op (add_mset (p, x) S) op'' \<Longrightarrow>
-   step io (set'_op S op) op'"
-  apply (subst set'_op.code)
-  apply (clarsimp del: disjCI split: op.splits simp flip: cin.rep_eq; hypsubst_thin?)
-  apply(rule Silent_in_choices_step, drule step_choicesE; simp)
-  by force
-
-lemma step_set_op_intro_Tau_2[intro]:
-  "io = Tau \<Longrightarrow>
-   step Tau op op'' \<Longrightarrow>
-   op' = set'_op S op'' \<Longrightarrow>
-   step io (set'_op S op) op'"
-  apply (subst set'_op.code)
-  apply (subst set'_op.code)
-  apply (clarsimp del: disjCI split: op.splits simp flip: cin.rep_eq; hypsubst_thin?)
-  apply (metis (no_types, lifting) IO.distinct(5) IO.simps(6) cimageI cinsertI1 op.simps(20) step.simps step_choicesE)
-  done
-*)
-
 (*source'_op *)
 
-definition source'_op_aux where
-  "source'_op_aux inps op = (case op of Read p f \<Rightarrow> cimage (\<lambda> x. (Inl o Inl) (p,f,x)) (acset (set_mset (inps p))) | op' \<Rightarrow> csingle ((Inl o Inr) op'))"
-
-corec source'_op where
-  "source'_op inps op = Choice (cimage (case_sum 
-    (\<lambda> op'. case op' of
-    Inl (p,f,x) \<Rightarrow> Silent (source'_op (inps(p := remove1_mset x (inps p))) (f x))
-  | Inr (Write op p x) \<Rightarrow> Write (source'_op inps op) p x
-  | Inr (Silent op) \<Rightarrow> Silent (source'_op inps op)) 
-    (\<lambda> p. Read p (\<lambda> x. source'_op (inps(p := add_mset x (inps p))) op)))
-  (cUn (cim Inr cUNIV) (cUnion (cim (source'_op_aux inps) (choices op)))))"
+corec source'_op :: "('a \<Rightarrow> 'b llist) \<Rightarrow> ('a, 'c, 'b) op \<Rightarrow> ('a, 'c, 'b) op" where
+  "source'_op inps op = Choice (cimage (\<lambda> op'. case op' of
+    Read p f \<Rightarrow> Silent (source'_op (inps(p := ltl (inps p))) (f (lhd (inps p))))
+  | Write op p x \<Rightarrow> Write (source'_op inps op) p x
+  | Silent op \<Rightarrow> Silent (source'_op inps op))
+  (cfilter (\<lambda> op. case op of Read p f \<Rightarrow> inps p \<noteq> LNil | _ \<Rightarrow> True) (choices op)))"
 
 lemma step_source'_op_intro_Out[intro]:
   "io = Out p x \<Longrightarrow>
@@ -145,19 +81,7 @@ lemma step_source'_op_intro_Out[intro]:
    step io (source'_op inps op) op'"
   apply(subst source'_op.corec.code)
   apply(erule step_choicesE; simp)
-  apply(rule Write_in_choices_step)
-  apply(simp add: source'_op_aux_def Bex_def)
   by fastforce
-
-lemma step_source'_op_intro_Inp[intro]:
-  "io = Inp p x \<Longrightarrow>
-   op' = source'_op (inps(p := add_mset x (inps p))) op \<Longrightarrow>
-   step io (source'_op inps op) op'"
-  apply(subst source'_op.corec.code)
-  apply simp
-  apply(rule Read_in_choices_step)
-  apply(simp add: source'_op_aux_def Bex_def)
-  by(auto intro!: ext intro: arg_cong[where f = "\<lambda> f. source'_op f _"])
 
 lemma step_source'_op_intro_Tau_Tau[intro]:
   "io = Tau \<Longrightarrow>
@@ -166,58 +90,64 @@ lemma step_source'_op_intro_Tau_Tau[intro]:
    step io (source'_op inps op) op'"
   apply(subst source'_op.corec.code)
   apply(erule step_choicesE; simp)
-  apply(rule Silent_in_choices_step)
-  apply(simp add: source'_op_aux_def Bex_def)
   by fastforce
+
+lemma x_in_rcset_acset: "x \<in> rcset (acset {y. (p, y) \<in># S}) = (x \<in> {y. (p, y) \<in># S})"
+  apply(subgoal_tac "{y. (p, y) \<in># S} \<in> {A. countable A}")
+  subgoal
+    by simp
+  subgoal
+    apply(auto intro!: countable_finite simp only: mem_Collect_eq set_mset_def simp add: finite_nonzero_count)
+    using finite_nonzero_count[of S, THEN finite_filter[of _ "\<lambda> (p',_). p = p'"], THEN finite_imageI[of _ snd ]]
+    apply -
+    apply(simp only: mem_Collect_eq Set.filter_eq image_def Bex_def split: sum.split)
+    by auto
+  done
 
 lemma step_source'_op_intro_Tau_Inp[intro]:
   "io = Tau \<Longrightarrow>
-   step (Inp p x) op op'' \<Longrightarrow>
-   op' = source'_op (inps(p := remove1_mset x (inps p))) op'' \<Longrightarrow>
-   x \<in># inps p \<Longrightarrow>
+   step (Inp p (lhd (inps p))) op op'' \<Longrightarrow>
+   op' = source'_op (inps(p := ltl (inps p))) op'' \<Longrightarrow>
+   inps p \<noteq> LNil \<Longrightarrow>
    step io (source'_op inps op) op'"
   apply(subst source'_op.corec.code)
   apply(erule step_choicesE; simp)
-  apply(rule Silent_in_choices_step)
-  apply(simp add: source'_op_aux_def Bex_def)
   by fastforce
 
 lemma step_source'_op_elim:
   assumes "step io (source'_op inps op) op'"
   obtains p x op'' where "io = Out p x" "step (Out p x) op op''" "op' = source'_op inps op''"
-  | p x where "io = Inp p x" "op' = source'_op (inps(p := add_mset x (inps p))) op"
-  | p x op'' where "io = Tau" "x \<in># inps p" "step (Inp p x) op op''" "op' = source'_op (inps(p := remove1_mset x (inps p))) op''"  
+  | p x op'' where "io = Tau" "inps p \<noteq> LNil" "step (Inp p (lhd (inps p))) op op''" "op' = source'_op (inps(p := ltl (inps p))) op''"  
   | op'' where "io = Tau" "step Tau op op''" "op' = source'_op inps op''"
   using assms apply -
   apply atomize_elim
   apply(subst (asm) source'_op.corec.code)
-  apply (auto del: disjCI split: op.splits sum.splits dest!: no_Choice_in_choices[simplified cin.rep_eq[symmetric]] Write_in_choices_step  simp flip: cin.rep_eq simp add: source'_op_aux_def ; hypsubst_thin?)
-    apply fastforce+
+  apply (auto del: disjCI split: op.splits sum.splits dest!: no_Choice_in_choices[simplified cin.rep_eq[symmetric]] Write_in_choices_step  simp flip: cin.rep_eq ; hypsubst_thin?)
+                 apply blast+
   done
 
-
 definition op_wrapper where     
-  "op_wrapper f_xs S op = set'_op S (source'_op f_xs op)"
+  "op_wrapper inps S op = set'_op S (source'_op inps op)"
 
 lemma step_op_wrapper_elim: 
-  assumes "step io (op_wrapper f_xs S op) op'" 
-  obtains p x where "io = Out p x" "(p, x) \<in># S" "op' = op_wrapper f_xs (remove1_mset (p, x) S) op" | 
-         p x op'' where "io = Tau" "step (Inp p x) op op''" "op' = op_wrapper (f_xs(p := (remove1_mset x (f_xs p)))) S op''" |
-         p x op'' where "io = Tau" "step (Out p x) op op''" "op' = op_wrapper f_xs (add_mset (p, x) S) op''" |
-         op'' where "io = Tau" "step Tau op op''" "op' = op_wrapper f_xs S op''"
+  assumes "step io (op_wrapper inps S op) op'" 
+  obtains p x where "io = Out p x" "(p, x) \<in># S" "op' = op_wrapper inps (remove1_mset (p, x) S) op" | 
+         p x op'' where "io = Tau" "step (Inp p (lhd (inps p))) op op''" "inps p \<noteq> LNil" "op' = op_wrapper (inps(p := ltl (inps p))) S op''" |
+         p x op'' where "io = Tau" "step (Out p x) op op''" "op' = op_wrapper inps (add_mset (p, x) S) op''" |
+         op'' where "io = Tau" "step Tau op op''" "op' = op_wrapper inps S op''"
   using assms
   unfolding op_wrapper_def
   apply -
-  by(blast elim!: step_set'_op_elim step_source'_op_elim)
+  by(auto elim!: step_set'_op_elim step_source'_op_elim)
 
-lemma step_op_wrapper_intro_Out[intro]:
+lemma step_op_wrapper_intro_Out:
   "io = Out p x \<Longrightarrow> (p, x) \<in># S \<Longrightarrow>
    op' = (op_wrapper inps (remove1_mset (p, x) S) op) \<Longrightarrow>
    step io (op_wrapper inps S op) op'"
   unfolding op_wrapper_def
   by auto
 
-lemma step_op_wrapper_intro_Tau_Tau[intro]:
+lemma step_op_wrapper_intro_Tau_Tau:
   "io = Tau \<Longrightarrow>
    step Tau op op'' \<Longrightarrow>
    op' = op_wrapper inps S op'' \<Longrightarrow>
@@ -225,32 +155,22 @@ lemma step_op_wrapper_intro_Tau_Tau[intro]:
   unfolding op_wrapper_def
   by auto
 
-lemma step_op_wrapper_intro_Tau_Inp[intro]:
+lemma step_op_wrapper_intro_Tau_Inp:
   "io = Tau \<Longrightarrow>
-   x \<in># inps p \<Longrightarrow>
-   step (Inp p x) op op'' \<Longrightarrow>
-   op' = op_wrapper (inps(p := remove1_mset x (inps p))) S op'' \<Longrightarrow>
+   inps p \<noteq> LNil \<Longrightarrow>
+   step (Inp p (lhd (inps p))) op op'' \<Longrightarrow>
+   op' = op_wrapper (inps(p := ltl (inps p))) S op'' \<Longrightarrow>
    step io (op_wrapper inps S op) op'"
   unfolding op_wrapper_def
   by auto
 
-lemma step_op_wrapper_intro_Tau_Out[intro]:
+lemma step_op_wrapper_intro_Tau_Out:
   "io = Tau \<Longrightarrow>
    step (Out p x) op op'' \<Longrightarrow>
-   op' = op_wrapper inps (add_mset (p, x) S) op'' \<Longrightarrow>
-   step io (op_wrapper inps S op) op'"
+   op' = op_wrapper S_in (add_mset (p, x) S_out) op'' \<Longrightarrow>
+   step io (op_wrapper S_in S_out op) op'"
   unfolding op_wrapper_def
   by auto
-
-definition init_conf' where 
-  "init_conf' chns f_xs S dt =
-  \<lparr> msg = \<lambda> _ _. empty_mset,
-    prog_msg = \<lambda> _ _. [],
-    ops = \<lambda> w. op_wrapper (f_xs w) (S w) (compile_dataflow_dis w chns dt),
-    used_wire = \<lambda> _. None \<rparr>"
-
-abbreviation conf_instance where
-  "conf_instance ws f_xs S op \<equiv> (init_conf' ws (\<lambda> w e. case e of Some (Inl e') \<Rightarrow> image_mset Inr (f_xs e' w) | _ \<Rightarrow> empty_mset) (\<lambda> w. (image_mset (\<lambda> (x,y). (Some (w,x), Inr y)) (S w))) op)"
 
 setup_lifting type_definition_multiset
 
@@ -314,89 +234,448 @@ proof -
 qed
 
 end
+(*
+lemma Test_case_Out: "io = Out (p1, p2) (x1, x2) \<Longrightarrow>
+    op = op_wrapper (bind_mset UNIV S_in) (remove1_mset ((p1, p2), x1, x2) (bind_mset UNIV S_out)) (compile_dataflow ws (dataflow_dis_transfer dt)) \<Longrightarrow>
+    ((p1, p2), x1, x2) \<in># S_out w \<Longrightarrow>
+    \<exists>c'. step_dis' (Out (p1, p2) (x1, x2)) (conf_instance ws S_in S_out dt) c' \<and>
+         (\<exists>S_in' S_out'.
+             op_wrapper (bind_mset UNIV S_in) (remove1_mset ((p1, p2), x1, x2) (bind_mset UNIV S_out)) (compile_dataflow ws (dataflow_dis_transfer dt)) =
+             op_wrapper (bind_mset UNIV S_in') (bind_mset UNIV S_out') (compile_dataflow ws (dataflow_dis_transfer dt)) \<and>
+             c' = conf_instance ws S_in' S_out' dt)"
+    apply(rule exI[where x = "conf_instance ws S_in (\<lambda>wa. if wa = w then remove1_mset ((p1, p2), x1, x2) (S_out w) else S_out wa) dt"])
+    apply(rule conjI)
+    subgoal
+      apply(rule step_dis'.intros[of w])
+      apply(rule step_dis.intros; (simp add: init_conf'_def))
+       apply(rule step_op_wrapper_intro_Out; (simp add: image_def))
+      subgoal
+        by force
+      by(auto split: prod.split simp add: image_mset_remove1_mset_if)
+    subgoal
+      apply(rule exI[where x = "S_in"])
+      apply(rule exI[where x = "S_out(w := remove1_mset ((p1, p2), x1, x2) (S_out w))"])
+      by auto
+    done
 
-lemma "(op_wrapper (\<lambda> x. bind_mset UNIV (f_xs x)) (bind_mset UNIV S) (compile_dataflow ws (Logic (tmap_op ip op os f) t_msg))) ~d 
-      conf_instance ws f_xs S (Logic_Dis (tmap_op ip op os f) t_msg pact)"
-proof (coinduction arbitrary: f_xs S os t_msg)
-  fix f_xs :: "'a \<times> 'b \<Rightarrow> 'e \<Rightarrow> ('c \<times> 'd) multiset"
-    and os :: "('b, 'c, 'f, 'g, 'd, 'h) operator_state_ty2_scheme"
-    and t_msg :: "'b \<Rightarrow> 'b \<Rightarrow> 'd buf"
-    and S :: "'e \<Rightarrow> (('a \<times> 'b) \<times> 'c \<times> 'd) multiset"
+lemma Test_case_Out_Logic: "io = Out (p1, p2) (x1, x2) \<Longrightarrow>
+    op = op_wrapper (bind_mset UNIV S_in) (remove1_mset ((p1, p2), x1, x2) (bind_mset UNIV S_out)) (compile_dataflow ws (Logic (dt ipp opp os f) t_msg)) \<Longrightarrow>
+    ((p1, p2), x1, x2) \<in># S_out w \<Longrightarrow>
+    \<exists>c'. step_dis' (Out (p1, p2) (x1, x2)) (conf_instance ws S_in S_out (Logic_Dis (dt ipp opp os f) t_msg pact)) c' \<and>
+         (\<exists>S_in' S_out' os' t_msg'.
+             op_wrapper (bind_mset UNIV S_in) (remove1_mset ((p1, p2), x1, x2) (bind_mset UNIV S_out)) (compile_dataflow ws (Logic (dt ipp opp os f) t_msg)) =
+             op_wrapper (bind_mset UNIV S_in') (bind_mset UNIV S_out') (compile_dataflow ws (Logic (dt ipp opp os' f) t_msg')) \<and>
+             c' = conf_instance ws S_in' S_out' (Logic_Dis (dt ipp opp os' f) t_msg' pact))"
+  using Test_case_Out[where dt = "Logic_Dis (dt ipp opp os f) t_msg pact"]
+  by fastforce
+
+(*
+lemma Test_case_Inp: "io = Tau \<Longrightarrow>
+    step (Inp (p1, p2) (x1, x2)) (compile_dataflow ws (Logic (dt ipp opp os f) t_msg)) op' \<Longrightarrow>
+    op = op_wrapper (remove1_mset ((p1, p2), x1, x2) (bind_mset UNIV S_in)) (bind_mset UNIV S_out) op' \<Longrightarrow>
+    \<exists>c'. step_dis' Tau (conf_instance ws S_in S_out (Logic_Dis (dt ipp opp os f) t_msg pact)) c' \<and>
+         (\<exists>S_in' S_out' os' t_msg'.
+             op_wrapper (remove1_mset ((p1, p2), x1, x2) (bind_mset UNIV S_in)) (bind_mset UNIV S_out) op' = op_wrapper (bind_mset UNIV S_in') (bind_mset UNIV S_out') (compile_dataflow ws (Logic (dt ipp opp os' f) t_msg')) \<and>
+             c' = conf_instance ws S_in' S_out' (Logic_Dis (dt ipp opp os' f) t_msg' pact))"
+  apply(rule exI[where x = "conf_instance ws (map_entry undefined (remove1_mset ((p1, p2), x1, x2)) S_out) S_out (Logic_Dis (dt ipp opp os f) t_msg pact)"])
+  apply(rule conjI)
+  subgoal
+    sorry
+  subgoal
+    unfolding compile_dataflow_def dataflow_tree_to_operator_def
+    apply simp
+    apply(erule step_dataflow_op_elim; simp)
+    apply(erule step_map_op_elim; simp)
+    apply(rule exI[where x = "S_in(undefined := remove1_mset ((p1, p2), x1, x2) (S_in undefined))"])
+    apply(rule exI[where x = "S_out"])
+    apply(rule exI[where x = "os"])
+    apply(rule exI[where x = "t_msg"])
+    apply auto
+    subgoal for io' op''
+      apply(cases io'; (auto split: option.splits))
+    sorry
+  done
+*)
+*)
+
+
+
+(*Not needed by work do it not work*)
+instantiation cset :: (enum) enum
+begin
+
+definition
+  enum_cset :: "'a cset buf" where
+    "enum_cset = undefined"
+
+definition
+  enum_all_cset :: "('a cset \<Rightarrow> bool) \<Rightarrow> bool" where
+    "enum_all_cset f = undefined"
+
+definition
+  enum_ex_cset :: "('a cset \<Rightarrow> bool) \<Rightarrow> bool" where
+    "enum_ex_cset f = undefined"
+
+instance
+  sorry
+(*sketch doesn't work ? ?*)
+end
+
+lemma csome_elem_single[simp] : "csome_elem {| x |} = x"
+  by(auto simp add: csome_elem_def)
+
+definition "init_exchange_conf =
+   \<lparr> c_temp = [],
+     c_glob = [] \<rparr>"
+
+definition "compile_dataflow_dis w chns dt temp' glob' = (let summary = dataflow_dis_tree_to_graph dt in
+                                    let op = snd (dataflow_dis_tree_to_operator w chns dt) in
+                                    let sg = init_subgraph summary (map (\<lambda> (nid, p). (Loc nid (Src p), bot, 1)) (List.product Enum.enum Enum.enum)) in
+                                    dataflow_dis_op sg (exchange_conf_one.make temp' glob') op)"
+
+definition init_conf' where 
+  "init_conf' chns S_in S_out temp' glob' dt =
+  \<lparr> msg = \<lambda> _ _. empty_mset,
+    prog_msg = \<lambda> _ _. [],
+    ops = \<lambda> w. op_wrapper (S_in w) (S_out w) (compile_dataflow_dis w chns (dt w) temp' glob'),
+    used_wire = \<lambda> _. None \<rparr>"
+
+abbreviation conf_instance where
+  "conf_instance ws inps S temp' glob' op \<equiv> (init_conf' ws  (\<lambda> w. case_option LNil (case_sum (\<lambda> p. lmap Inr (inps w p)) (\<lambda> _. LNil))) (\<lambda> w. (image_mset (\<lambda> (x,y). (Some (w,x), Inr y)) (S w))) temp' glob' op)"
+
+definition "init_subgraph_ext summary pt_tr' upfro' =
+   \<lparr> pt_tr = pt_tr',
+   edges = graph_to_edges summary,
+   summ = summary, upfro = upfro' \<rparr>"
+
+definition "compile_dataflow_ext chns pt_tr' upfro' dt = (let summary = dataflow_tree_to_graph dt in
+                                    let op = dataflow_tree_to_operator chns dt in
+                                    let sg = init_subgraph_ext summary pt_tr' upfro' in
+                                    dataflow_op sg op)"
+
+definition "compile_dataflow_dis_ext w chns dt pt_tr' upfro' temp' glob' = (let summary = dataflow_dis_tree_to_graph dt in
+                                    let op = snd (dataflow_dis_tree_to_operator w chns dt) in
+                                    let sg = init_subgraph_ext summary pt_tr' upfro' in
+                                    dataflow_dis_op sg (exchange_conf_one.make temp' glob') op)"
+
+definition init_conf'_ext where 
+  "init_conf'_ext chns S_in S_out dt pt_tr' upfro' temp' glob' =
+  \<lparr> msg = \<lambda> _ _. empty_mset,
+    prog_msg = \<lambda> _ _. [],
+    ops = \<lambda> w. op_wrapper (S_in w) (S_out w) (compile_dataflow_dis_ext w chns (dt w) (pt_tr' w) (upfro' w) temp' glob'),
+    used_wire = \<lambda> _. None \<rparr>"
+
+abbreviation conf_instance_ext where
+  "conf_instance_ext ws inps S pt_tr' upfro' temp' glob' op \<equiv> 
+  (init_conf'_ext ws (\<lambda> w. case_option LNil (case_sum (\<lambda> p. lmap Inr (inps w p)) (\<lambda> _. LNil))) 
+  (\<lambda> w. (image_mset (\<lambda> (x,y). (Some (w,x), Inr y)) (S w))) op pt_tr' upfro' temp' glob')"
+
+lemma dataflow_tree_to_graph_op_invariant: "dataflow_tree_to_graph (Logic op t_msg) = dataflow_tree_to_graph (Logic op' t_msg)"
+  by(auto simp add: dataflow_tree_to_graph_def)
+
+(* My undefined invariant and all the theorems i want to be true about it *)
+definition invar where
+  "invar inps inpss S Ss os oss pt_tr' pt_trs' upfro' upfros' temp' glob' in_out_rel = undefined"
+
+(*
+lemma invar_theorem1: "invar inps inpss S Ss (os :: (_,_,_) operator_state) (oss :: _ \<Rightarrow> (_,_,_) operator_state) \<Longrightarrow> inps p \<noteq> LNil \<Longrightarrow> lhd (inps (0, ipp)) = (d, t) \<Longrightarrow> invar (inps(p := ltl (inps p))) inpss S Ss (consumes os p t d) oss"
+*)
+lemma invar_theorem1: "invar inps inpss S Ss os oss pt_tr' pt_trs' upfro' upfros' temp' glob' in_out_rel \<Longrightarrow> inps p \<noteq> LNil \<Longrightarrow> lhd (inps p) = (d, t) \<Longrightarrow> 
+                       invar (inps(p := ltl (inps p))) inpss S Ss (consumes os (snd p) t d) oss pt_tr' pt_trs' upfro' upfros' temp' glob' in_out_rel"
+  sorry
+
+lemma invar_theorem2: "invar inps inpss S Ss os oss pt_tr' pt_trs' upfro' upfros' temp' glob' in_out_rel \<Longrightarrow> initia os \<Longrightarrow> outpu os (snd p) = x # xs \<Longrightarrow> 
+                       invar inps inpss (add_mset (p, x) S) Ss (os\<lparr>outpu := (outpu os)(snd p := xs)\<rparr>) oss pt_tr' pt_trs' upfro' upfros' temp' glob' in_out_rel"
+  sorry
+
+lemma invar_theorem3: "invar inps inpss S Ss os oss pt_tr' pt_trs' upfro' upfros' temp' glob' in_out_rel \<Longrightarrow>
+    initia os \<Longrightarrow>
+    has_progress os \<Longrightarrow>
+    (os', st) = obtain_progress os \<Longrightarrow>
+    invar inps inpss S Ss os' oss
+     (change_multiplicities (dataflow_tree_to_graph (Logic op t_msg))
+       (extract_progress nid (graph_to_edges (dataflow_tree_to_graph (Logic op t_msg))) st) pt_tr')
+     pt_trs' (\<lambda>_. True) upfros' temp' glob' in_out_rel"
+  sorry
+
+lemma invar_theorem4: "
+    upfro' n \<Longrightarrow>
+    propagate_all
+     (dataflow_tree_to_graph
+       (Logic (builder_op b ipp opp os (logic ipp opp)) t_msg))
+     pt_tr' =
+    Some pt_tr_new \<Longrightarrow>
+    \<not> initia os \<Longrightarrow>
+    invar inps inpss S Ss
+     (os\<lparr>front := frontier \<circ> (\<lambda>p. c_imp pt_tr_new (Loc n (Trg p))), initia := True,
+           nfron := True\<rparr>)
+     oss pt_tr_new pt_trs' (upfro'(n := False)) upfros' temp' glob' in_out_rel"
+
+
+lemma Case2: "step (Inp p (lhd (inps p))) (compile_dataflow_ext ws pt_tr' upfro' (Logic (builder_op b ipp opp os (logic ipp opp)) t_msg)) op' \<Longrightarrow>
+    invar inps inpss S Ss os oss pt_tr' pt_trs' upfro' upfros' temp' glob' in_out_rel \<Longrightarrow> inps p \<noteq> LNil \<Longrightarrow>
+    \<exists>c'. wstep_dis Tau (conf_instance_ext ws inpss Ss pt_trs' upfros' temp' glob' (\<lambda>w. Logic_Dis (builder_op b ipp opp (oss w) (logic ipp opp)) t_msg pact)) c' \<and>
+         (\<exists>inps' inpss' S' Ss' os' oss' pt_tr'' pt_trs'' upfro'' upfros'' temp'' glob''.
+             op_wrapper (inps(p := ltl (inps p))) S op' =
+             op_wrapper inps' S' (compile_dataflow_ext ws pt_tr'' upfro'' (Logic (builder_op b ipp opp os' (logic ipp opp)) t_msg)) \<and>
+             (c' = conf_instance_ext ws inpss' Ss' pt_trs'' upfros'' temp'' glob'' (\<lambda>w. Logic_Dis (builder_op b ipp opp (oss' w) (logic ipp opp)) t_msg pact) \<and>
+                 invar inps' inpss' S' Ss' os' oss' pt_tr'' pt_trs'' upfro'' upfros'' temp'' glob'' in_out_rel))"
+  apply(rule exI[where x = "conf_instance_ext ws inpss Ss pt_trs' upfros' temp' glob' (\<lambda>w. Logic_Dis (builder_op b ipp opp (oss w) (logic ipp opp)) t_msg pact)"])
+  apply(auto dest!: map_IO_elim elim!: step_builder_op_elim step_map_op_elim step_dataflow_op_elim 
+      simp add: compile_dataflow_ext_def wstep_dis_refl dataflow_tree_to_operator_def split: option.splits)
+  subgoal for p' x1 x2
+    apply(rule exI[where x = "map_entry (0, p') ltl inps"])
+    apply(rule exI[where x = "inpss"])
+    apply(rule exI[where x = "S"])
+    apply(rule exI[where x = "Ss"])
+    apply(rule exI[where x = "consumes os p' x2 x1"])
+    apply(rule exI[where x = "oss"])
+    apply(rule exI[where x = "pt_tr'"])
+    apply(rule exI[where x = "pt_trs'"])
+    apply(rule exI[where x = "upfro'"])
+    apply(rule conjI)
+    subgoal
+      using dataflow_tree_to_graph_op_invariant
+      by metis
+    subgoal
+      apply(rule exI[where x = "upfros'"])
+      apply(rule exI[where x = "temp'"])
+      apply(rule exI[where x = "glob'"])
+      using invar_theorem1
+      by fastforce
+    done
+  done
+
+lemma Case3: "step (Out p x) (compile_dataflow_ext ws pt_tr' upfro' (Logic (builder_op b ipp opp os (logic ipp opp)) t_msg)) op' \<Longrightarrow>
+    invar inps inpss S Ss os oss pt_tr' pt_trs' upfro' upfros' temp' glob' in_out_rel \<Longrightarrow>
+    \<exists>c'. wstep_dis Tau
+          (conf_instance_ext ws inpss Ss pt_trs' upfros' temp' glob'
+            (\<lambda>w. Logic_Dis (builder_op b ipp opp (oss w) (logic ipp opp)) t_msg pact))
+          c' \<and>
+         (\<exists>inps' inpss' S' Ss' os' oss' pt_tr'' pt_trs'' upfro''.
+             op_wrapper inps (add_mset (p, x) S) op' =
+             op_wrapper inps' S' (compile_dataflow_ext ws pt_tr'' upfro'' (Logic (builder_op b ipp opp os' (logic ipp opp)) t_msg)) \<and>
+             (\<exists>upfros'' temp'' glob''.
+                 c' =
+                 conf_instance_ext ws inpss' Ss' pt_trs'' upfros'' temp'' glob''
+                  (\<lambda>w. Logic_Dis (builder_op b ipp opp (oss' w) (logic ipp opp)) t_msg pact) \<and>
+                 invar inps' inpss' S' Ss' os' oss' pt_tr'' pt_trs'' upfro'' upfros'' temp'' glob'' in_out_rel))"
+  apply(rule exI[where x = "conf_instance_ext ws inpss Ss pt_trs' upfros' temp' glob' (\<lambda>w. Logic_Dis (builder_op b ipp opp (oss w) (logic ipp opp)) t_msg pact)"])
+  apply(auto dest!: map_IO_elim elim!: step_builder_op_elim step_map_op_elim step_dataflow_op_elim 
+      simp add: compile_dataflow_ext_def wstep_dis_refl dataflow_tree_to_operator_def split: option.splits)
+  subgoal for p' x1 x2 xs
+    apply(rule exI[where x = "inps"])
+    apply(rule exI[where x = "inpss"])
+    apply(rule exI[where x = "add_mset ((0, p'), x1, x2) S"])
+    apply(rule exI[where x = "Ss"])
+    apply(rule exI[where x = "os\<lparr>outpu := (outpu os)(p' := xs)\<rparr>"])
+    apply(rule exI[where x = "oss"])
+    apply(rule exI[where x = "pt_tr'"])
+    apply(rule exI[where x = "pt_trs'"])
+    apply(rule exI[where x = "upfro'"])
+    apply(rule conjI)
+    subgoal
+      using dataflow_tree_to_graph_op_invariant
+      by metis
+    subgoal
+      apply(rule exI[where x = "upfros'"])
+      apply(rule exI[where x = "temp'"])
+      apply(rule exI[where x = "glob'"])
+      using invar_theorem2
+      by fastforce
+    done
+  done
+
+lemma Case4: "step io (builder_op b ipp opp os (logic ipp opp)) op'' \<Longrightarrow>
+     map_IO (case_option (Inl 0) (\<lambda>p. Inr (0, p))) (case_option (Inl 0) (\<lambda>p. Inr (0, p))) id io = Out (Inl nid) (Inl (Inl st)) \<Longrightarrow>
+    invar inps inpss S Ss os oss (pt_tr' :: (('g :: {enum,minus,one,plus,zero,hashable,linorder}, _) location, _) configuration) pt_trs' upfro' upfros' temp' glob' in_out_rel \<Longrightarrow>
+    \<exists>c'. wstep_dis Tau (conf_instance_ext ws inpss Ss pt_trs' upfros' temp' glob' (\<lambda>w. Logic_Dis (builder_op b ipp opp (oss w) (logic ipp opp)) t_msg pact)) c' \<and>
+         (\<exists>inps' inpss' S' Ss' os' oss' (pt_tr'' :: (('g, _) location, _) configuration) pt_trs'' upfro''.
+             op_wrapper inps S
+              (dataflow_op
+                (init_subgraph_ext (dataflow_tree_to_graph (Logic (builder_op b ipp opp os (logic ipp opp)) t_msg)) pt_tr' upfro'
+                 \<lparr>upfro := \<lambda>_. True,
+                    pt_tr :=
+                      change_multiplicities (summ (init_subgraph_ext (dataflow_tree_to_graph (Logic (builder_op b ipp opp os (logic ipp opp)) t_msg)) pt_tr' upfro'))
+                       (extract_progress nid (edges (init_subgraph_ext (dataflow_tree_to_graph (Logic (builder_op b ipp opp os (logic ipp opp)) t_msg)) pt_tr' upfro')) st)
+                       (pt_tr (init_subgraph_ext (dataflow_tree_to_graph (Logic (builder_op b ipp opp os (logic ipp opp)) t_msg)) pt_tr' upfro'))\<rparr>)
+                (map_op (case_option (Inl 0) (\<lambda>p. Inr (0, p))) (case_option (Inl 0) (\<lambda>p. Inr (0, p))) op'')) =
+             op_wrapper inps' S'
+              (dataflow_op (init_subgraph_ext (dataflow_tree_to_graph (Logic (builder_op b ipp opp os' (logic ipp opp)) t_msg)) pt_tr'' upfro'')
+                (map_op (case_option (Inl 0) (\<lambda>p. Inr (0, p))) (case_option (Inl 0) (\<lambda>p. Inr (0, p))) (builder_op b ipp opp os' (logic ipp opp)))) \<and>
+             (\<exists>upfros'' temp'' glob''.
+                 c' = conf_instance_ext ws inpss' Ss' pt_trs'' upfros'' temp'' glob'' (\<lambda>w. Logic_Dis (builder_op b ipp opp (oss' w) (logic ipp opp)) t_msg pact) \<and>
+                 invar inps' inpss' S' Ss' os' oss' pt_tr'' pt_trs'' upfro'' upfros'' temp'' glob'' in_out_rel))"
+          apply(auto dest!: map_IO_elim elim!: step_builder_op_elim simp add: tmap_op_def split: option.splits)
+          subgoal for os'
+            apply(rule exI[where x = "conf_instance_ext ws inpss Ss pt_trs' upfros' temp' glob' (\<lambda>w. Logic_Dis (builder_op b ipp opp (oss w) (logic ipp opp)) t_msg pact)"])
+            apply(simp add: wstep_dis_refl)
+            apply(rule exI[where x = "inps"])
+            apply(rule exI[where x = "inpss"])
+            apply(rule exI[where x = "S"])
+            apply(rule exI[where x = "Ss"])
+            apply(rule exI[where x = "os'"])
+            apply(rule exI[where x = "oss"])
+            apply(rule exI[where x = "change_multiplicities (dataflow_tree_to_graph (Logic (builder_op b ipp opp os (logic ipp opp)) t_msg))
+     (extract_progress 0 (graph_to_edges (dataflow_tree_to_graph (Logic (builder_op b ipp opp os (logic ipp opp)) t_msg))) st) pt_tr'"])
+            apply(rule exI[where x = "pt_trs'"])
+            apply(rule exI[where x = "(\<lambda>_. True)"])
+            apply(rule conjI)
+            subgoal
+              apply(rule arg_cong[where f = "\<lambda> os. op_wrapper _ _ (dataflow_op os _)"])
+              unfolding init_subgraph_ext_def
+              apply auto
+              subgoal
+                unfolding obtain_progress_def 
+                using dataflow_tree_to_graph_op_invariant
+                by metis
+              subgoal
+                unfolding obtain_progress_def graph_to_edges_def dataflow_tree_to_graph_def
+                by fastforce
+              done
+            apply(rule exI[where x = "upfros'"])
+            apply(rule exI[where x = "temp'"])
+            apply(rule exI[where x = "glob'"])
+            apply auto
+            using invar_theorem3
+            by fast
+          done
+
+
+
+(*TODO TODO instead of using bisim_dis use one that uses wstep instead of step, since we want to not take an action (or multiple) TODO TODO*)
+(*TODO TODO make a condition between inps and inpss maybe using countable multisets? and for os and oss TODO TODO*)
+lemma "invar inps inpss S Ss os oss pt_tr' pt_trs' upfro' upfros' temp' glob' in_out_rel \<Longrightarrow> (op_wrapper inps S (compile_dataflow_ext ws pt_tr' upfro' (Logic (tmap_op ipp opp (os :: (_,_,_,_,_) operator_state_ty2) f) t_msg))) ~dw 
+      conf_instance_ext ws inpss Ss pt_trs' upfros' temp' glob' (\<lambda> w. (Logic_Dis (tmap_op ipp opp ((oss :: 'w :: enum \<Rightarrow> (_,_,_,_,_) operator_state_ty2) w) f) t_msg pact)) "
+proof (coinduction arbitrary: inps inpss S Ss os oss pt_tr' pt_trs' upfro' upfros' temp' glob')
+  fix   inps :: "'a \<times> 'b \<Rightarrow> ('c \<times> 'd) llist"
+    and inpss :: "'w \<Rightarrow> 'a \<times> 'b \<Rightarrow> ('c \<times> 'd) llist"
+    and S :: "(('a \<times> 'b) \<times> 'c \<times> 'd) multiset"
+    and Ss :: "'w \<Rightarrow> (('a \<times> 'b) \<times> 'c \<times> 'd) multiset"
+    and os :: "('b, 'c, 'e, 'f, 'd) operator_state_ty2"
+    and oss :: "'w \<Rightarrow> ('b, 'c, 'e, 'f, 'd) operator_state_ty2"
+    and pt_tr' :: "(('a, 'b) location, 'd) configuration"
+    and pt_trs' :: "'w \<Rightarrow> (('a, 'b) location, 'd) configuration"
+    and upfro' :: "'a \<Rightarrow> bool"
+    and upfros' :: "'w \<Rightarrow> 'a \<Rightarrow> bool"
+    and temp' :: "(('a, 'b) location \<times> 'd \<times> int) buf"
+    and glob' :: "(('a, 'b) location \<times> 'd \<times> int) buf"
+  assume invar: "invar inps inpss S Ss os oss pt_tr' pt_trs' upfro' upfros' temp' glob' in_out_rel"
 (* TODO try to see if local definition makes things more readable
   define op1 where "op1 = (\<lambda> f_xs S S' os t_msg. op_wrapper (\<lambda>x. bind_mset UNIV (f_xs x)) (cUNION cUNIV S) (cUNION cUNIV S') (compile_dataflow ws (Logic (tmap_op ip op os f) t_msg)))"
 *)
-  let ?op1 = "\<lambda> f_xs S os t_msg. op_wrapper (\<lambda>x. bind_mset UNIV (f_xs x)) (bind_mset UNIV S) (compile_dataflow ws (Logic (tmap_op ip op os f) t_msg))"
-  let ?c1 = "\<lambda> f_xs S os t_msg. conf_instance ws f_xs S (Logic_Dis (tmap_op ip op os f) t_msg pact)"
+  let ?op1 = "\<lambda> inps S os pt_tr' upfro'. op_wrapper inps S (compile_dataflow_ext ws pt_tr' upfro' (Logic (tmap_op ipp opp (os :: (_,_,_,_,_) operator_state_ty2) f) t_msg))"
+  let ?c1 = "\<lambda> inpss Ss oss pt_trs' upfros' temp' glob'. conf_instance_ext ws inpss Ss pt_trs' upfros' temp' glob' (\<lambda> w. (Logic_Dis (tmap_op ipp opp (oss w) f) t_msg pact))"
 (*
   let ?c1 = "\<lambda> f_xs S S' os t_msg. init_conf' ws (\<lambda>w. case_option {#} (case_sum (\<lambda>e'. Inr `# f_xs e' w) (\<lambda>b. {#}))) (\<lambda>w. (\<lambda>(x, y). (Some (w, x), Inr y)) |`| S w) (\<lambda>w. (\<lambda>(x, y). (Some (w, x), Inr y)) |`| S' w) (Logic_Dis (tmap_op ip op os f) t_msg pact)"
 *)
-  have "sim_dis (\<lambda>uu uua. (\<exists>f_xs S (os :: ('b, 'c, 'f, 'g, 'd, 'h) operator_state_ty2_scheme) t_msg. uu = ?op1 f_xs S os t_msg \<and> uua = ?c1 f_xs S os t_msg)) (?op1 f_xs S os t_msg) (?c1 f_xs S os t_msg)"
-    unfolding sim_dis_def
+  have "wsim_dis (\<lambda>op c. (\<exists> inps inpss S Ss (os :: (_,_,_,_,_) operator_state_ty2) (oss :: _ \<Rightarrow> (_,_,_,_,_) operator_state_ty2) pt_tr' pt_trs' upfro' upfros' temp' glob'. 
+    op = ?op1 inps S os pt_tr' upfro' \<and> c = ?c1 inpss Ss oss pt_trs' upfros' temp' glob' \<and> invar inps inpss S Ss os oss pt_tr' pt_trs' upfro' upfros' temp' glob' in_out_rel)) (?op1 inps S os pt_tr' upfro') (?c1 inpss Ss oss pt_trs' upfros' temp' glob')"
+    unfolding wsim_dis_def
     apply simp
     apply safe
     subgoal for io op
       apply(drule step_op_wrapper_elim; simp)
       apply safe
-      subgoal for p1 p2 x1 x2 w
-        apply(rule exI[where x = "undefined"])
-        apply(rule conjI)
-        subgoal
-          sorry
-        subgoal
-          apply(rule exI[where x = "f_xs"])
-          apply(rule exI[where x = "S(w := remove1_mset ((p1, p2), x1, x2) (S w))"])
-          apply(rule exI[where x = "os"])
-          apply(rule exI[where x = "t_msg"])
-          apply auto
-
+      (* Case where an element is written from the multiset S, use something like Test_case_Out_Logic*)
+      subgoal for p1 p2 d t
         sorry
-      subgoal
-        sorry
-      subgoal
-        sorry
+      (* Case where dataflow_op read an element from inps - Done - Relies on invar_theorem1*)
+      subgoal for p1 p2 op'
+        using invar Case2
+        unfolding tmap_op_def
+        by fast
+      (* Case where dataflow_op write an element to S - Done - Relies on invar_theorem2*)
+      subgoal for p1 p2 x1 x2 op'
+        using invar Case3
+        unfolding tmap_op_def
+        by fastforce
+      (* Case where dataflow_op makes a Tau step*)
       subgoal for op'
-        unfolding compile_dataflow_def dataflow_tree_to_operator_def
-        apply simp
-        apply(erule step_dataflow_op_elim; simp)
+        apply(simp add: compile_dataflow_ext_def)
+        apply(erule step_dataflow_op_elim; simp add: dataflow_tree_to_operator_def; erule step_map_op_elim; simp?)
+        (* Case where the build_op's logic is applied*)
+(*
+        subgoal premises prems for op''
+*)
         subgoal for op''
-          apply(erule step_map_op_elim)
-          apply safe
-          apply(erule step_tmap_op_elim; simp?)
-          subgoal for io' op''' os'
+          apply(erule thin_rl)
+          apply(erule HOL.cnf.weakening_thm)
+          apply(erule HOL.cnf.weakening_thm)
+(*
+          unfolding tmap_op_def
+          apply(erule step_builder_op_elim; simp)
+          subgoal for os'
+            apply(erule HOL.cnf.weakening_thm[where P = "op'' = _"])
+            apply(subst (asm) tmap_logic_def)
+            apply simp
+            apply(erule HOL.cnf.weakening_thm[where P = "os' = _"])
+            apply(rule exI[where x = "conf_instance ws inpss Ss (\<lambda>w. Logic_Dis (builder_op False {|ipp|} {|opp|} (oss w) (tmap_logic ipp opp f)) t_msg pact)"])
+            apply(simp add: wstep_dis_refl)
+            apply(rule exI[where x = "inps"])
+            apply(rule exI[where x = "inpss"])
+            apply(rule exI[where x = "S"])
+            apply(rule exI[where x = "Ss"])
+*)
+          sorry
+        (* Case where ...*)
+        subgoal for nid st io op''
+          unfolding tmap_op_def
+          using Case4 invar
+          by fast
+        (* Case where ...*)
+        subgoal for nid imp_fron sg' io' op''
+          apply(erule HOL.cnf.weakening_thm)
+          apply(erule HOL.cnf.weakening_thm)
+          apply(erule HOL.cnf.weakening_thm)
+          apply(erule HOL.cnf.weakening_thm[where P = "imp_fron = _"])
+          apply(erule HOL.cnf.weakening_thm[where P = "op' = _"])
+          apply(subst (asm) init_subgraph_ext_def; simp)
+          apply(auto dest!: map_IO_elim elim!: step_builder_op_elim simp add: tmap_op_def split: option.splits)
+          subgoal for pt_tr_new
+            apply(erule HOL.cnf.weakening_thm[where P = "io' = _"])
+            apply(erule HOL.cnf.weakening_thm[where P = "nid = _"])
+            apply(erule HOL.cnf.weakening_thm[where P = "op'' = _"])
+            apply(subst (asm) init_subgraph_ext_def; simp)
+            apply(subst (asm) init_subgraph_ext_def; simp)
+            unfolding init_subgraph_ext_def
+            apply(simp)
+            unfolding init_subgraph_ext_def[symmetric]
+            apply(rule exI[where x = "conf_instance_ext ws inpss Ss pt_trs' upfros' temp' glob'
+            (\<lambda>w. Logic_Dis (builder_op False {|ipp|} {|opp|} (oss w) (tmap_logic ipp opp f))
+                   t_msg pact)"])
+            apply(simp add: wstep_dis_refl)
+            apply(rule exI[where x = "inps"])
+            apply(rule exI[where x = "inpss"])
+            apply(rule exI[where x = "S"])
+            apply(rule exI[where x = "Ss"])
+            apply(rule exI[where x = "os\<lparr>front := frontier \<circ> (\<lambda>p. c_imp pt_tr_new (Loc 0 (Trg p))), initia := True,
+                    nfron := True\<rparr>"])
+            apply(rule exI[where x = "oss"])
+            apply(rule exI[where x = "pt_tr_new"])
+            apply(rule exI[where x = "pt_trs'"])
+            apply(rule exI[where x = "upfro'(0 := False)"])
+            apply(rule conjI)
+            subgoal
+              using dataflow_tree_to_graph_op_invariant
+              by metis
+            apply(rule exI[where x = "upfros'"])
+            apply(rule exI[where x = "temp'"])
+            apply(rule exI[where x = "glob'"])
+            apply simp
 
-end
-          apply auto
-          apply(rule exI[where x = "?c1 f_xs S S' os t_msg"]; simp)
-          apply safe
-          subgoal for op'''
+            
             sorry
-          subgoal for op'''
-            apply(rule exI[where x = f_xs])
-            apply(rule exI[where x = S])
-            apply(rule exI[where x = S'])
-            apply(rule exI[where x = os])
-            apply(rule exI[where x = t_msg])
-            apply auto
-            apply(erule step_tmap_op_elim; simp?)
-            sorry
-          done
-        subgoal
-          sorry
-        subgoal
-          sorry
         done
       done
     subgoal for io op
-      apply(drule step_dis'_elim, erule exE)
-      subgoal for w
-        apply(drule step_dis_elim)
       sorry
     done
-  done
-  then show "\<exists>opa c. ?op1 f_xs S S' os t_msg = opa \<and> ?c1 f_xs S S' os t_msg = c \<and> 
-      sim_dis (\<lambda>uu uua. (\<exists>f_xs S S' (os :: ('b, 'c, 'f, 'g, 'd, 'h) operator_state_ty2_scheme) t_msg. uu = ?op1 f_xs S S' os t_msg \<and> uua = ?c1 f_xs S S' os t_msg) \<or> uu ~d uua) opa c"
+  then show "\<exists>op c. ?op1 inps S os pt_tr' upfro' = op \<and> ?c1 inpss Ss oss pt_trs' upfros' temp' glob' = c \<and>
+    wsim_dis (\<lambda>op c. (\<exists>inps inpss S Ss (os :: (_,_,_,_,_) operator_state_ty2) (oss :: _ \<Rightarrow> (_,_,_,_,_) operator_state_ty2) pt_tr' pt_trs' upfro' upfros' temp' glob'.
+       op = ?op1 inps S os pt_tr' upfro' \<and> c = ?c1 inpss Ss oss pt_trs' upfros' temp' glob' \<and> invar inps inpss S Ss os oss pt_tr' pt_trs' upfro' upfros' temp' glob' in_out_rel) \<or> op ~dw c) op c"
     apply simp
-    apply(rule predicate2D[OF sim_dis_mono, rotated], assumption)
+    apply(rule predicate2D[OF wsim_dis_mono, rotated], assumption)
     by blast
   qed
 
